progress backwards simulation: changed definition of inhale to be more direct (no indirection via a plus operator) and also made inhale a relation on single states

TotalExpressions.thy
@@ -1,5 +1,5 @@
 theory TotalExpressions
-imports Viper.ViperLang Viper.ValueAndBasicState TotalViperState Viper.Binop
+imports Viper.ViperLang Viper.ValueAndBasicState TotalViperState Viper.Binop Viper.DeBruijn
 begin
 
 (* duplicated: TODO share it *)
@@ -11,66 +11,97 @@ fun the_rat :: "'a val \<Rightarrow> rat" where
   "the_rat (VPerm r) = r"
 | "the_rat _ = undefined"
 
-(* not sure about this notation *)
-fun red_pure_exp_total :: "program \<Rightarrow> pure_exp \<Rightarrow> 'a full_total_state \<Rightarrow> 'a val"
-  ("_ \<turnstile> ((\<langle>_;_\<rangle>) [\<Down>]\<^sub>t)" [51,0,0] 81)
-  where 
-  "Pr \<turnstile> \<langle>ELit l; _\<rangle> [\<Down>]\<^sub>t = (val_of_lit l)"
-| "Pr \<turnstile> \<langle>Var n; (\<sigma>, _, _)\<rangle> [\<Down>]\<^sub>t = the (\<sigma> n)"
-| "Pr \<turnstile> \<langle>Unop unop e; \<omega>\<rangle> [\<Down>]\<^sub>t = the (eval_unop unop (Pr \<turnstile> \<langle>e;\<omega>\<rangle> [\<Down>]\<^sub>t))"
-| "Pr \<turnstile> \<langle>Binop e1 bop e2; \<omega>\<rangle> [\<Down>]\<^sub>t = (let v1 = (Pr \<turnstile> \<langle>e1; \<omega>\<rangle> [\<Down>]\<^sub>t) in let r = eval_binop_lazy v1 bop in
-  if r \<noteq> None then the r else the (eval_binop v1 bop (Pr \<turnstile> \<langle>e2; \<omega>\<rangle> [\<Down>]\<^sub>t)))"
-| "Pr \<turnstile> \<langle>CondExp e1 e2 e3; \<omega>\<rangle> [\<Down>]\<^sub>t = (if (Pr \<turnstile> \<langle>e1; \<omega>\<rangle> [\<Down>]\<^sub>t = VBool True) then (Pr \<turnstile> \<langle>e2; \<omega>\<rangle> [\<Down>]\<^sub>t) else (Pr \<turnstile> \<langle>e3; \<omega>\<rangle> [\<Down>]\<^sub>t))"
-(* difference to virtual state: heap lookup *)
-| "Pr \<turnstile> \<langle>FieldAcc e f; \<omega>\<rangle> [\<Down>]\<^sub>t = get_heap_total_full \<omega> (the_address (Pr \<turnstile> \<langle>e; \<omega>\<rangle> [\<Down>]\<^sub>t), f)"
-| "Pr \<turnstile> \<langle>Old l e; (\<sigma>, \<tau>, \<phi>)\<rangle> [\<Down>]\<^sub>t = (Pr \<turnstile> \<langle>e; (\<sigma>, \<tau>, (the (\<tau> l)))\<rangle> [\<Down>]\<^sub>t)"
-| "Pr \<turnstile> \<langle>Perm e f; \<omega>\<rangle> [\<Down>]\<^sub>t = VPerm (Rep_prat (get_mask_total_full \<omega> ((the_address (Pr \<turnstile> \<langle>e; \<omega>\<rangle> [\<Down>]\<^sub>t)), f)))"
+inductive red_pure_exp_total :: "program \<Rightarrow> 'a interp \<Rightarrow> pure_exp \<Rightarrow> 'a full_total_state \<Rightarrow> 'a extended_val \<Rightarrow> bool"
+  ("_, _ \<turnstile> ((\<langle>_;_\<rangle>) [\<Down>]\<^sub>t _)" [51,51,0,51,51] 81)
+  where
+(* Independent of SA *)
+  RedLit: "Pr, \<Delta> \<turnstile> \<langle>ELit l; _\<rangle> [\<Down>]\<^sub>t Val (val_of_lit l)"
+| RedVar: "\<lbrakk> \<sigma> n = Some v \<rbrakk> \<Longrightarrow> Pr, \<Delta> \<turnstile> \<langle>Var n; (\<sigma>, _, _)\<rangle> [\<Down>]\<^sub>t Val v"
+| RedUnop: "\<lbrakk> Pr, \<Delta> \<turnstile> \<langle>e; \<omega>\<rangle> [\<Down>]\<^sub>t Val v ; eval_unop unop v = Some v' \<rbrakk> \<Longrightarrow> Pr, \<Delta> \<turnstile> \<langle>Unop unop e; \<omega>\<rangle> [\<Down>]\<^sub>t Val v'"
+| RedBinopLazy: "\<lbrakk> Pr, \<Delta> \<turnstile> \<langle>e1; \<omega>\<rangle> [\<Down>]\<^sub>t Val v1 ; eval_binop_lazy v1 bop = Some v \<rbrakk>
+  \<Longrightarrow> Pr, \<Delta> \<turnstile> \<langle>Binop e1 bop e2; \<omega>\<rangle> [\<Down>]\<^sub>t Val v"
+| RedBinop: "\<lbrakk> Pr, \<Delta> \<turnstile> \<langle>e1; \<omega>\<rangle> [\<Down>]\<^sub>t Val v1 ; Pr, \<Delta> \<turnstile> \<langle>e2; \<omega>\<rangle> [\<Down>]\<^sub>t Val v2 ; eval_binop_lazy v1 bop = None; eval_binop v1 bop v2 = Some v \<rbrakk>
+  \<Longrightarrow> Pr, \<Delta> \<turnstile> \<langle>Binop e1 bop e2; \<omega>\<rangle> [\<Down>]\<^sub>t Val v"
+(*| RedOld: "\<lbrakk> t l = Some \<phi> ; Pr, \<Delta> \<turnstile> \<langle>e; (\<sigma>, t, \<phi>)\<rangle> [\<Down>]\<^sub>t v \<rbrakk> \<Longrightarrow> Pr, \<Delta> \<turnstile> \<langle>Old l e; (\<sigma>, t, _)\<rangle> [\<Down>]\<^sub>t v"*) (* Implicitly propagates failures *)
+(*| RedLet: "\<lbrakk> Pr, \<Delta> \<turnstile> \<langle>e1; \<omega>\<rangle> [\<Down>]\<^sub>t Val v1 ; Pr, \<Delta> \<turnstile> \<langle>e2; shift_and_add_state \<omega> v1\<rangle> [\<Down>]\<^sub>t r \<rbrakk> \<Longrightarrow> Pr, \<Delta> \<turnstile> \<langle>Let e1 e2; \<omega>\<rangle> [\<Down>]\<^sub>t r"
+| RedExistsTrue: "\<lbrakk> v \<in> set_from_type \<Delta> ty ; Pr, \<Delta> \<turnstile> \<langle>e; shift_and_add_state \<omega> v\<rangle> [\<Down>]\<^sub>t Val (VBool True) ;
+  \<And>v'. \<exists>b. Pr, \<Delta> \<turnstile> \<langle>e; shift_and_add_state \<omega> v'\<rangle> [\<Down>]\<^sub>t Val (VBool b) \<rbrakk>
+  \<Longrightarrow> Pr, \<Delta> \<turnstile> \<langle>PExists ty e; \<omega>\<rangle> [\<Down>]\<^sub>t Val (VBool True)"
+| RedExistsFalse: "\<lbrakk> \<And>v. v \<in> set_from_type \<Delta> ty \<longrightarrow> Pr, \<Delta> \<turnstile> \<langle>e; shift_and_add_state \<omega> v\<rangle> [\<Down>]\<^sub>t Val (VBool False) \<rbrakk>
+  \<Longrightarrow> Pr, \<Delta> \<turnstile> \<langle>PExists ty e; \<omega>\<rangle> [\<Down>]\<^sub>t Val (VBool False)"
+| RedForallTrue: "\<lbrakk> \<And>v. v \<in> set_from_type \<Delta> ty \<longrightarrow> Pr, \<Delta> \<turnstile> \<langle>e; shift_and_add_state \<omega> v\<rangle> [\<Down>]\<^sub>t Val (VBool True) \<rbrakk>
+  \<Longrightarrow> Pr, \<Delta> \<turnstile> \<langle>PForall ty e; \<omega>\<rangle> [\<Down>]\<^sub>t Val (VBool True)"
+| RedForallFalse: "\<lbrakk> v \<in> set_from_type \<Delta> ty ; Pr, \<Delta> \<turnstile> \<langle>e; shift_and_add_state \<omega> v\<rangle> [\<Down>]\<^sub>t Val (VBool False) \<rbrakk>
+  \<Longrightarrow> Pr, \<Delta> \<turnstile> \<langle>PForall ty e; \<omega>\<rangle> [\<Down>]\<^sub>t Val (VBool False)"*)
+| RedCondExpTrue: "\<lbrakk> Pr, \<Delta> \<turnstile> \<langle>e1; \<omega>\<rangle> [\<Down>]\<^sub>t Val (VBool True) ; Pr, \<Delta> \<turnstile> \<langle>e2; \<omega>\<rangle> [\<Down>]\<^sub>t r \<rbrakk>
+  \<Longrightarrow> Pr, \<Delta> \<turnstile> \<langle>CondExp e1 e2 e3; \<omega>\<rangle> [\<Down>]\<^sub>t r"
+| RedCondExpFalse: "\<lbrakk> Pr, \<Delta> \<turnstile> \<langle>e1; \<omega>\<rangle> [\<Down>]\<^sub>t Val (VBool False) ; Pr, \<Delta> \<turnstile> \<langle>e3; \<omega>\<rangle> [\<Down>]\<^sub>t r \<rbrakk>
+  \<Longrightarrow> Pr, \<Delta> \<turnstile> \<langle>CondExp e1 e2 e3; \<omega>\<rangle> [\<Down>]\<^sub>t r"
+| RedPermNull: "\<lbrakk> Pr, \<Delta> \<turnstile> \<langle>e; \<omega>\<rangle> [\<Down>]\<^sub>t Val (VRef Null) \<rbrakk> \<Longrightarrow> Pr, \<Delta> \<turnstile> \<langle>Perm e f; \<omega>\<rangle> [\<Down>]\<^sub>t Val (VPerm 0)"
+| RedResult: "\<lbrakk> \<sigma> 0 = Some v \<rbrakk> \<Longrightarrow> Pr, \<Delta> \<turnstile> \<langle>Result; (\<sigma>, _, _)\<rangle> [\<Down>]\<^sub>t Val v"
+(*| RedUnfoldingPermNegFailure: "\<lbrakk> Pr, \<Delta> \<turnstile> \<langle>f; \<omega>\<rangle> [\<Down>]\<^sub>t Val (VPerm v) ; v < 0 \<rbrakk> \<Longrightarrow> Pr, \<Delta> \<turnstile> \<langle>Unfolding p exps f e; \<omega>\<rangle> [\<Down>]\<^sub>t VFailure"*)
 
-(*| "Pr \<turnstile> \<langle>PermPred p exps; \<omega>\<rangle> [\<Down>]\<^sub>t = VPerm (get_pm \<omega> (p, List.map (\<lambda>e. conf, Pr, \<Delta> \<turnstile> \<langle>e; \<omega>\<rangle> [\<Down>]\<^sub>t) exps))" *)
-
+| RedBinopRightFailure: "\<lbrakk> Pr, \<Delta> \<turnstile> \<langle>e1; \<omega>\<rangle> [\<Down>]\<^sub>t Val v1 ; Pr, \<Delta> \<turnstile> \<langle>e2; \<omega>\<rangle> [\<Down>]\<^sub>t VFailure ;  eval_binop_lazy v1 bop = None \<rbrakk>
+  \<Longrightarrow> Pr, \<Delta> \<turnstile> \<langle>Binop e1 bop e2; \<omega>\<rangle> [\<Down>]\<^sub>t VFailure"
+| RedBinopFailure: "\<lbrakk> Pr, \<Delta> \<turnstile> \<langle>e1; \<omega>\<rangle> [\<Down>]\<^sub>t Val v1 ; Pr, \<Delta> \<turnstile> \<langle>e2; \<omega>\<rangle> [\<Down>]\<^sub>t Val v2 ; eval_binop v1 bop v2 = None ; eval_binop_lazy v1 bop = None \<rbrakk>
+  \<Longrightarrow> Pr, \<Delta> \<turnstile> \<langle>Binop e1 bop e2; \<omega>\<rangle> [\<Down>]\<^sub>t VFailure" (* Division by 0 *)
+| RedOldFailure: "\<lbrakk> t l = None \<rbrakk> \<Longrightarrow> Pr, \<Delta> \<turnstile> \<langle>Old l e ; (_, t, _)\<rangle> [\<Down>]\<^sub>t VFailure"
 (*
-| "conf, Pr, \<Delta> \<turnstile> \<langle>FunApp f exps; \<omega>\<rangle> [\<Down>]\<^sub>t = the (the (funs \<Delta> f) (List.map (\<lambda>e. conf, Pr, \<Delta> \<turnstile> \<langle>e; \<omega>\<rangle> [\<Down>]\<^sub>t) exps) (get_v \<omega>))"
-| "conf, Pr, \<Delta> \<turnstile> \<langle>Result; (\<sigma>, _, _)\<rangle> [\<Down>]\<^sub>t = the (\<sigma> 0)"
+| RedExistsFailure: "\<lbrakk> v \<in> set_from_type \<Delta> ty \<longrightarrow> Pr, \<Delta> \<turnstile> \<langle>e; shift_and_add_state \<omega> v\<rangle> [\<Down>]\<^sub>t VFailure \<rbrakk>
+  \<Longrightarrow> Pr, \<Delta> \<turnstile> \<langle>PExists ty e; \<omega>\<rangle> [\<Down>]\<^sub>t VFailure"
+| RedForallFailure: "\<lbrakk> v \<in> set_from_type \<Delta> ty \<longrightarrow> Pr, \<Delta> \<turnstile> \<langle>e; shift_and_add_state \<omega> v\<rangle> [\<Down>]\<^sub>t VFailure \<rbrakk>
+  \<Longrightarrow> Pr, \<Delta> \<turnstile> \<langle>PForall ty e; \<omega>\<rangle> [\<Down>]\<^sub>t VFailure"*)
+| RedPropagateFailure: "\<lbrakk> e \<in> sub_pure_exp e' ; Pr, \<Delta> \<turnstile> \<langle>e; \<omega>\<rangle> [\<Down>]\<^sub>t VFailure \<rbrakk> \<Longrightarrow>  Pr, \<Delta> \<turnstile> \<langle>e'; \<omega>\<rangle> [\<Down>]\<^sub>t VFailure"
 
-| "conf, Pr, \<Delta> \<turnstile> \<langle>Unfolding p exps f e; \<omega>\<rangle> [\<Down>]\<^sub>t = (if equi_predicate conf then (conf, Pr, \<Delta> \<turnstile> \<langle>e; \<omega>\<rangle> [\<Down>]\<^sub>t)
-  else (conf, Pr, \<Delta> \<turnstile> \<langle>e; (SOME \<omega>'. \<omega>' \<in> unfold_states conf Pr \<Delta> p (List.map (\<lambda>e. conf, Pr, \<Delta> \<turnstile> \<langle>e; \<omega>\<rangle> [\<Down>]\<^sub>t) exps) (the_rat (conf, Pr, \<Delta> \<turnstile> \<langle>f; \<omega>\<rangle> [\<Down>]\<^sub>t)) \<omega>)\<rangle> [\<Down>]\<^sub>t))"
-
-| "conf, Pr, \<Delta> \<turnstile> \<langle>Let e1 e2; \<omega>\<rangle> [\<Down>]\<^sub>t = (conf, Pr, \<Delta> \<turnstile> \<langle>e2; shift_and_add_state \<omega> (conf, Pr, \<Delta> \<turnstile> \<langle>e1; \<omega>\<rangle> [\<Down>]\<^sub>t)\<rangle> [\<Down>]\<^sub>t)"
-
-| "conf, Pr, \<Delta> \<turnstile> \<langle>PExists ty e; \<omega>\<rangle> [\<Down>]\<^sub>t = VBool (\<exists>v \<in> set_from_type \<Delta> ty. (conf, Pr, \<Delta> \<turnstile> \<langle>e; shift_and_add_state \<omega> v\<rangle> [\<Down>]\<^sub>t = VBool True))"
-| "conf, Pr, \<Delta> \<turnstile> \<langle>PForall ty e; \<omega>\<rangle> [\<Down>]\<^sub>t = VBool (\<forall>v \<in> set_from_type \<Delta> ty. (conf, Pr, \<Delta> \<turnstile> \<langle>e; shift_and_add_state \<omega> v\<rangle> [\<Down>]\<^sub>t = VBool True))"
+(* Dependent on the SA *)
+| RedField: "\<lbrakk> Pr, \<Delta> \<turnstile> \<langle>e; \<omega>\<rangle> [\<Down>]\<^sub>t Val (VRef (Address a)) ; get_heap_total_full \<phi> (a, f) = v \<rbrakk> \<Longrightarrow> Pr, \<Delta> \<turnstile> \<langle>FieldAcc e f; \<omega>\<rangle> [\<Down>]\<^sub>t Val v"
+| RedPerm: "\<lbrakk> Pr, \<Delta> \<turnstile> \<langle>e; \<omega>\<rangle> [\<Down>]\<^sub>t Val (VRef (Address a)) \<rbrakk> \<Longrightarrow> Pr, \<Delta> \<turnstile> \<langle>Perm e f; \<omega>\<rangle> [\<Down>]\<^sub>t Val (VPerm (Rep_prat (get_mask_total_full \<omega> (a, f))))"
+(*
+(* perm(P(...)) = 0 if equirecursive *)
+| RedPermPred: "\<lbrakk> list_all2 (\<lambda>e v. Pr, \<Delta> \<turnstile> \<langle>e; \<omega>\<rangle> [\<Down>] Val v) exps vals \<rbrakk>
+  \<Longrightarrow> Pr, \<Delta> \<turnstile> \<langle>PermPred p exps; \<omega>\<rangle> [\<Down>] Val (VPerm (Rep_prat (get_pm \<omega> (p, vals))))"
 *)
 
 datatype inh_exh_conf = CInhale | CExhale "heap_loc set"
 
+fun wd_binop :: "binop \<Rightarrow> 'a val \<Rightarrow> 'a val \<Rightarrow> bool"
+  where 
+    "wd_binop Div v1 v2 \<longleftrightarrow> v2 \<noteq> (VInt 0)"
+  | "wd_binop Mod v1 v2 \<longleftrightarrow> v2 \<noteq> (VInt 0)"
+  | "wd_binop _ _ _ = True"
 
-fun (sequential) wd_pure_exp_total :: "program \<Rightarrow> inh_exh_conf \<Rightarrow> pure_exp \<Rightarrow> 'a full_total_state \<Rightarrow> bool"
+(* can't show this, since need to take typing into account *)
+lemma wd_binop_total: 
+  assumes "wd_binop bop v1 v2"
+  shows "binop_eval v1 v2 \<noteq> None"
+  oops
+
+fun wd_pure_exp_total :: "program \<Rightarrow> 'a interp \<Rightarrow> inh_exh_conf \<Rightarrow> pure_exp \<Rightarrow> 'a full_total_state \<Rightarrow> bool"
   where
-(* TODO *)
-  "wd_pure_exp_total Pr c (ELit l) \<omega> \<longleftrightarrow> True"
-| "wd_pure_exp_total Pr c (Var n) \<omega> \<longleftrightarrow> True"
+  "wd_pure_exp_total Pr \<Delta> c (ELit l) \<omega> \<longleftrightarrow> True"
+| "wd_pure_exp_total Pr \<Delta> c (Var n) \<omega> \<longleftrightarrow> True"
+| "wd_pure_exp_total Pr \<Delta> c (Unop unop e) \<omega> \<longleftrightarrow> (wd_pure_exp_total Pr \<Delta> c e \<omega>)"
+| "wd_pure_exp_total Pr \<Delta> c (Binop e1 bop e2) \<omega> \<longleftrightarrow> 
+     (wd_pure_exp_total Pr \<Delta> c e1 \<omega> \<and> ((\<forall>v1. Pr, \<Delta> \<turnstile> \<langle>e1; \<omega>\<rangle> [\<Down>]\<^sub>t Val v1 \<longrightarrow> eval_binop_lazy v1 bop = None \<longrightarrow> 
+                  ((\<forall>v2. Pr, \<Delta> \<turnstile> \<langle>e2; \<omega>\<rangle> [\<Down>]\<^sub>t Val v2 \<longrightarrow> wd_binop bop v1 v2) \<and> (wd_pure_exp_total Pr \<Delta> c e2 \<omega>)))))"
+| "wd_pure_exp_total Pr \<Delta> c (CondExp e1 e2 e3) \<omega> \<longleftrightarrow> 
+     wd_pure_exp_total Pr \<Delta> c e1 \<omega> \<and> (if ((Pr,\<Delta> \<turnstile> \<langle>e1; \<omega>\<rangle> [\<Down>]\<^sub>t Val (VBool True))) then wd_pure_exp_total Pr \<Delta> c e2 \<omega> else wd_pure_exp_total Pr \<Delta> c e3 \<omega>)" 
+| "wd_pure_exp_total Pr \<Delta> CInhale (FieldAcc e f) \<omega> \<longleftrightarrow> 
+    wd_pure_exp_total Pr \<Delta> CInhale e \<omega> \<and> (\<forall>l. (Pr, \<Delta> \<turnstile> \<langle>e;\<omega>\<rangle> [\<Down>]\<^sub>t Val (VRef (Address l))) \<longrightarrow> (pgt (get_mask_total_full \<omega> (l,f)) pnone))"
+| "wd_pure_exp_total Pr \<Delta> (CExhale locs) (FieldAcc e f) \<omega> \<longleftrightarrow> 
+    (\<forall>l. ( (Pr,\<Delta> \<turnstile> \<langle>e;\<omega>\<rangle> [\<Down>]\<^sub>t Val (VRef (Address l))) \<longrightarrow> (l,f) \<in> locs))"
+| "wd_pure_exp_total Pr \<Delta> c (Perm e f) \<omega> \<longleftrightarrow> wd_pure_exp_total Pr \<Delta> c e \<omega> \<and> (\<forall>r. (Pr, \<Delta> \<turnstile> \<langle>e;\<omega>\<rangle> [\<Down>]\<^sub>t Val (VRef r)) \<longrightarrow> r \<noteq> Null)"
+| "wd_pure_exp_total Pr \<Delta> c _ _  \<longleftrightarrow> False"
 
-| "wd_pure_exp_total Pr c (Unop unop e) \<omega> \<longleftrightarrow> (wd_pure_exp_total Pr c e \<omega>)"
-| "wd_pure_exp_total Pr c (Binop e1 bop e2) \<omega> \<longleftrightarrow> 
-     (wd_pure_exp_total Pr c e1 \<omega> \<and> (let v1 = (Pr \<turnstile> \<langle>e1; \<omega>\<rangle> [\<Down>]\<^sub>t)
-          in eval_binop_lazy v1 bop = None \<longrightarrow> (wd_pure_exp_total Pr c e2 \<omega>)))"
-| "wd_pure_exp_total Pr c (CondExp e1 e2 e3) \<omega> \<longleftrightarrow> 
-     wd_pure_exp_total Pr c e1 \<omega> \<and> (if (un_VBool (Pr \<turnstile> \<langle>e1; \<omega>\<rangle> [\<Down>]\<^sub>t)) then wd_pure_exp_total Pr c e2 \<omega> else wd_pure_exp_total Pr c e3 \<omega>)" 
-| "wd_pure_exp_total Pr CInhale (FieldAcc e f) \<omega> \<longleftrightarrow> 
-    (let l = the_address (Pr \<turnstile> \<langle>e;\<omega>\<rangle> [\<Down>]\<^sub>t) in (pgt (get_mask_total_full \<omega> (l,f)) pnone))"
-| "wd_pure_exp_total Pr (CExhale locs) (FieldAcc e f) \<omega> \<longleftrightarrow> 
-    (let l = the_address (Pr \<turnstile> \<langle>e;\<omega>\<rangle> [\<Down>]\<^sub>t) in (l,f) \<in> locs)"
+(* TODO *)
 (*
-| "wd_pure_exp_total conf Pr \<Delta> (CondExp e1 e2 e3) \<omega> \<longleftrightarrow> wd_pure_exp_total conf Pr \<Delta> e1 \<and> (if  "
-| "wd_pure_exp_total conf Pr \<Delta> (FieldAcc e f) \<omega> \<longleftrightarrow> False"
-| "wd_pure_exp_total conf Pr \<Delta> (Old l e) \<omega> \<longleftrightarrow> False"
-| "wd_pure_exp_total conf Pr \<Delta> (Perm e f) \<omega> \<longleftrightarrow> False"
 | "wd_pure_exp_total conf Pr \<Delta> (PermPred p exps) \<omega> \<longleftrightarrow> False"
 | "wd_pure_exp_total conf Pr \<Delta> (FunApp f exps) \<omega> \<longleftrightarrow> False"
 | "wd_pure_exp_total conf Pr \<Delta> Result \<omega> \<longleftrightarrow> False"
 | "wd_pure_exp_total conf Pr \<Delta> (Unfolding p exps f e) \<omega> \<longleftrightarrow> False"
 | "wd_pure_exp_total conf Pr \<Delta> (Let e1 e2) \<omega> \<longleftrightarrow> False"
 | "wd_pure_exp_total conf Pr \<Delta> (PExists ty e) \<omega> \<longleftrightarrow> False"
-| "wd_pure_exp_total conf Pr \<Delta> (PForall ty e) \<omega> \<longleftrightarrow> False" *)
+| "wd_pure_exp_total conf Pr \<Delta> (PForall ty e) \<omega> \<longleftrightarrow> False" 
+*)
 
 end
